Improved error messages and documentation pertaining to certain ill-formed uses of syntaxp, in response to feedback from Robert Krug.

axioms.lisp
@@ -6705,52 +6705,47 @@
            (EQUAL (LXD X)
                   (LXD (NORM X)))).
   ~ev[]
-  The ~c[syntaxp] hypothesis in this rule will allow the rule to be
-  applied to ~c[(lxd (trn a b))] but will not allow it to be applied to
+  The ~c[syntaxp] hypothesis in this rule will allow the rule to be applied to
+  ~c[(lxd (trn a b))] but will not allow it to be applied to
   ~c[(lxd (norm a))].~/
   ~bv[]
   General Form:
   (SYNTAXP test)
   ~ev[]
-  ~c[Syntaxp] always returns ~c[t] and so may be added as a vacuous
-  hypothesis.  However, when relieving the hypothesis, the test
-  ``inside'' the ~c[syntaxp] form is actually treated as a meta-level
-  proposition about the proposed instantiation of the rule's variables
-  and that proposition must evaluate to true (non-~c[nil]) to
-  ``establish'' the ~c[syntaxp] hypothesis.
+  ~c[Syntaxp] always returns ~c[t] and so may be added as a vacuous hypothesis.
+  However, when relieving the hypothesis, the test ``inside'' the ~c[syntaxp]
+  form is actually treated as a meta-level proposition about the proposed
+  instantiation of the rule's variables and that proposition must evaluate to
+  true (non-~c[nil]) to ``establish'' the ~c[syntaxp] hypothesis.
 
-  Note that the test of a ~c[syntaxp] hypothesis does not, in general,
-  deal with the meaning or semantics or values of the terms, but rather
-  with their syntactic forms.  In the example above, the ~c[syntaxp]
-  hypothesis allows the rule to be applied to every target of the form
-  ~c[(lxd u)], provided ~c[u] is not of the form ~c[(norm v)].
-  Observe that without this syntactic restriction the rule above could
-  loop producing a sequence of increasingly complex targets ~c[(lxd a)],
-  ~c[(lxd (norm a))], ~c[(lxd (norm (norm a)))], etc.  An intuitive reading
-  of the rule might be ``~c[norm] the argument of ~c[lxd] unless it has
-  already been ~c[norm]ed.''
+  Note that the test of a ~c[syntaxp] hypothesis does not, in general, deal
+  with the meaning or semantics or values of the terms, but rather with their
+  syntactic forms.  In the example above, the ~c[syntaxp] hypothesis allows the
+  rule to be applied to every target of the form ~c[(lxd u)], provided ~c[u] is
+  not of the form ~c[(norm v)].  Observe that without this syntactic
+  restriction the rule above could loop, producing a sequence of increasingly
+  complex targets ~c[(lxd a)], ~c[(lxd (norm a))], ~c[(lxd (norm (norm a)))],
+  etc.  An intuitive reading of the rule might be ``~c[norm] the argument of
+  ~c[lxd] unless it has already been ~c[norm]ed.''
 
-  Note also that a ~c[syntaxp] hypothesis deals with the syntactic
-  form used internally by ACL2, rather than that seen by the user.  In
-  some cases these are the same, but there can be subtle differences
-  with which the writer of a ~c[syntaxp] hypothesis must be aware.
-  You can use ~c[:]~ilc[trans] to display this internal representation.
+  Note also that a ~c[syntaxp] hypothesis deals with the syntactic form used
+  internally by ACL2, rather than that seen by the user.  In some cases these
+  are the same, but there can be subtle differences with which the writer of a
+  ~c[syntaxp] hypothesis must be aware.  You can use ~c[:]~ilc[trans] to
+  display this internal representation.
 
-  There are two types of ~c[syntaxp] hypotheses.  The simpler type of
-  ~c[syntaxp] hypothesis may be used as the nth hypothesis in a
-  ~c[:]~ilc[rewrite] or ~c[:]~ilc[linear] rule whose ~c[:]~ilc[corollary] is
-  ~c[(implies (and hyp1 ... hypn ... hypk) (equiv lhs rhs))]
-  provided ~c[test] is a term, ~c[test] contains at least one variable, and
-  every variable occuring freely in ~c[test] occurs freely in ~c[lhs] or in
-  some ~c[hypi], ~c[i<n].  In addition, ~c[test] must not use any
-  stobjs.  The case of ~c[:]~ilc[meta] rules is similar to the above, except
-  that it applies to the result of applying the hypothesis metafunction.
-  (Later below we will describe the second type, an ~em[extended] ~c[syntaxp]
-  hypothesis, which may use ~ilc[state].)
+  There are two types of ~c[syntaxp] hypotheses.  The simpler type may be a
+  hypothesis of a ~c[:]~ilc[rewrite] or ~c[:]~ilc[linear] rule provided
+  ~c[test] contains at least one variable but no free variables
+  (~pl[free-variables]).  In particular, ~c[test] may not use ~il[stobj]s; any
+  stobj name will be treated as an ordinary variable.  The case of
+  ~c[:]~ilc[meta] rules is similar to the above, except that it applies to the
+  result of applying the hypothesis metafunction.  (Later below we will
+  describe the second type, an ~em[extended] ~c[syntaxp] hypothesis, which may
+  use ~ilc[state].)
 
   We illustrate the use of simple ~c[syntaxp] hypotheses by slightly
-  elaborating the example given above.  Consider a ~c[:]~ilc[rewrite]
-  rule whose ~c[:]~ilc[corollary] is:
+  elaborating the example given above.  Consider a ~c[:]~ilc[rewrite] rule:
   ~bv[]
   (IMPLIES (AND (RATIONALP X)
                 (SYNTAXP (NOT (AND (CONSP X)
@@ -6759,46 +6754,45 @@
                   (LXD (NORM X))))
   ~ev[]
   How is this rule applied to ~c[(lxd (trn a b))]?  First, we form a
-  substitution that instantiates the left-hand side of the conclusion
-  of the rule so that it is identical to the target term.  In the
-  present case, the substitution replaces ~c[x] with ~c[(trn a b)].
+  substitution that instantiates the left-hand side of the conclusion of the
+  rule so that it is identical to the target term.  In the present case, the
+  substitution replaces ~c[x] with ~c[(trn a b)].
   ~bv[]
   (LXD X) ==> (LXD (trn a b)).
   ~ev[]
   Then we backchain to establish the hypotheses, in order.  Ordinarily this
-  means that we instantiate each hypothesis with our substitution and
-  then attempt to rewrite the resulting instance to true.
-  Thus, in order to relieve the first hypothesis above, we rewrite
+  means that we instantiate each hypothesis with our substitution and then
+  attempt to rewrite the resulting instance to true.  Thus, in order to relieve
+  the first hypothesis above, we rewrite
   ~bv[]
   (RATIONALP (trn a b)).
   ~ev[]
   If this rewrites to true, we continue.
 
-  Of course, most users are aware of some exceptions to this general
-  description of the way we relieve hypotheses.  For
-  example, if a hypothesis contains a ``free-variable'' ~-[] one not
-  bound by the current substitution ~-[] we attempt to extend the
-  substitution by searching for an instance of the hypothesis among
-  known truths.  ~l[free-variables].  ~ilc[Force]d hypotheses are another exception to the
-  general rule of how hypotheses are relieved.
+  Of course, many users are aware of some exceptions to this general
+  description of the way we relieve hypotheses.  For example, if a hypothesis
+  contains a ``free-variable'' ~-[] one not bound by the current substitution
+  ~-[] we attempt to extend the substitution by searching for an instance of
+  the hypothesis among known truths.  ~l[free-variables].  ~ilc[Force]d
+  hypotheses are another exception to the general rule of how hypotheses are
+  relieved.
 
-  Hypotheses marked with ~c[syntaxp], as in ~c[(syntaxp test)], are
-  also exceptions.  We instantiate such a hypothesis; but instead of
-  rewriting the instantiated instance, we evaluate the instantiated
-  ~c[test].  More precisely, we evaluate ~c[test] in an environment in
-  which its variable symbols are bound to the quotations of the terms
-  to which those variables are bound in the instantiating
-  substitution.  So in the case in point, we (in essence) evaluate
+  Hypotheses marked with ~c[syntaxp], as in ~c[(syntaxp test)], are also
+  exceptions.  We instantiate such a hypothesis; but instead of rewriting the
+  instantiated instance, we evaluate the instantiated ~c[test].  More
+  precisely, we evaluate ~c[test] in an environment in which its variable
+  symbols are bound to the quotations of the terms to which those variables are
+  bound in the instantiating substitution.  So in the case in point, we (in
+  essence) evaluate
   ~bv[]
   (NOT (AND (CONSP '(trn a b)) (EQ (CAR '(trn a b)) 'NORM))).
   ~ev[]
-  This clearly evaluates to ~c[t].  When a ~c[syntaxp] test evaluates
-  to true, we consider the ~c[syntaxp] hypothesis to have been
-  established; this is sound because logically ~c[(syntaxp test)] is
-  ~c[t] regardless of ~c[test].  If the test evaluates to ~c[nil] (or
-  fails to evaluate because of ~il[guard] violations) we act as though
-  we cannot establish the hypothesis and abandon the attempt to apply
-  the rule; it is always sound to give up.
+  This clearly evaluates to ~c[t].  When a ~c[syntaxp] test evaluates to true,
+  we consider the ~c[syntaxp] hypothesis to have been established; this is
+  sound because logically ~c[(syntaxp test)] is ~c[t] regardless of ~c[test].
+  If the test evaluates to ~c[nil] (or fails to evaluate because of ~il[guard]
+  violations) we act as though we cannot establish the hypothesis and abandon
+  the attempt to apply the rule; it is always sound to give up.
 
   The acute reader will have noticed something odd about the form
   ~bv[]
@@ -6807,16 +6801,15 @@
   When relieving the first hypothesis, ~c[(RATIONALP X)], we substituted
   ~c[(trn a b)] for ~c[X]; but when relieving the second hypothesis,
   ~c[(SYNTAXP (NOT (AND (CONSP X) (EQ (CAR X) 'NORM))))], we substituted the
-  quotation of ~c[(trn a b)] for ~c[X].  Why the difference?  Remember
-  that in the first hypothesis we are talking about the value of
-  ~c[(trn a b)] ~-[] is it rational ~-[] while in the second one we are
-  talking about its syntactic form.  Remember also that Lisp, and hence
-  ACL2, evaluates the arguments to a function before applying the function
-  to the resulting values. Thus, we are asking ``Is the list ~c[(trn a b)]
-  a ~ilc[consp] and if so, is its ~ilc[car] the symbol ~c[NORM]?''  The
-  ~c[quote]s on both ~c[(trn a b)] and ~c[NORM] are therefore necessary.
-  One can verify this by defining ~c[trn] to be, say ~ilc[cons], and then
-  evaluating forms such as
+  quotation of ~c[(trn a b)] for ~c[X].  Why the difference?  Remember that in
+  the first hypothesis we are talking about the value of ~c[(trn a b)] ~-[] is
+  it rational ~-[] while in the second one we are talking about its syntactic
+  form.  Remember also that Lisp, and hence ACL2, evaluates the arguments to a
+  function before applying the function to the resulting values. Thus, we are
+  asking ``Is the list ~c[(trn a b)] a ~ilc[consp] and if so, is its ~ilc[car]
+  the symbol ~c[NORM]?''  The ~c[quote]s on both ~c[(trn a b)] and ~c[NORM] are
+  therefore necessary.  One can verify this by defining ~c[trn] to be, say
+  ~ilc[cons], and then evaluating forms such as
   ~bv[]
   (AND (CONSP '(trn a b)) (EQ (CAR '(trn a b)) 'NORM))
   (AND (CONSP (trn a b)) (EQ (CAR (trn a b)) NORM))
@@ -6827,16 +6820,98 @@
 
   ~l[syntaxp-examples] for more examples of the use of ~c[syntaxp].
 
-  An extended ~c[syntaxp] hypothesis is similar to the simple type
-  described above, but it uses two additional variables, ~c[mfc] and ~c[state],
-  which must not be bound by the left hand side or an earlier hypothesis
-  of the rule.  They must be the last two variables mentioned by ~c[form];
-  first ~c[mfc], then ~c[state].  These two variables give access to
-  the functions ~c[mfc-]xxx; ~pl[extended-metafunctions].  As
-  described there, ~c[mfc] is bound to the so-called
-  metafunction-context and ~c[state] to ACL2's ~ilc[state].
-  ~l[syntaxp-examples] for an example of the use of these extended
-  ~c[syntaxp] hypotheses."
+  An extended ~c[syntaxp] hypothesis is similar to the simple type described
+  above, but it uses two additional variables, ~c[mfc] and ~c[state], which
+  must not be bound by the left hand side or an earlier hypothesis of the rule.
+  They must be the last two variables mentioned by ~c[form]; first ~c[mfc],
+  then ~c[state].  These two variables give access to the functions
+  ~c[mfc-]xxx; ~pl[extended-metafunctions].  As described there, ~c[mfc] is
+  bound to the so-called metafunction-context and ~c[state] to ACL2's
+  ~ilc[state].  ~l[syntaxp-examples] for an example of the use of these
+  extended ~c[syntaxp] hypotheses.
+
+  We conclude with an example illustrating an error that may occur if you
+  forget that a ~c[syntaxp] hypothesis will be evaluated in an environment
+  where variables are bound to syntactic terms, not to values.  Consider the
+  following ~il[stobj] introduction (~pl[defstobj]).
+  ~bv[]
+    (defstobj st
+      (fld1 :type (signed-byte 3) :initially 0)
+      fld2)
+  ~ev[]
+  The following ~c[syntaxp] hypothesis is ill-formed for evaluation.  Indeed,
+  ACL2 causes an error because it anticipates that when trying to relieve the
+  ~c[syntaxp] hypothesis of this rule, ACL2 would be evaluating ~c[(fld1 st)]
+  where ~c[st] is bound to a term, not to an actual ~c[stobj] as required by
+  the function ~c[fld1].  The error message is intended to explain this
+  problem.
+  ~bv[]
+    ACL2 !>(defthm bad
+             (implies (syntaxp (quotep (fld1 st)))
+                      (equal (stp st)
+                             (and (true-listp st)
+                                  (equal (len st) 2)
+                                  (fld1p (car st))))))
+
+
+    ACL2 Error in ( DEFTHM BAD ...):  The form (QUOTEP (FLD1 ST)), from
+    a SYNTAXP hypothesis, is not suitable for evaluation in an environment
+    where its variables are bound to terms.  See :DOC SYNTAXP.  Here is
+    further explanation:
+         The form ST is being used, as an argument to a call of FLD1, where
+    the single-threaded object of that name is required.  But in the current
+    context, the only declared stobj name is STATE.  Note:  this error
+    occurred in the context (FLD1 ST).
+
+
+    Summary
+    Form:  ( DEFTHM BAD ...)
+    Rules: NIL
+    Time:  0.00 seconds (prove: 0.00, print: 0.00, other: 0.00)
+
+    ACL2 Error in ( DEFTHM BAD ...):  See :DOC failure.
+
+    ******** FAILED ********
+    ACL2 !>
+  ~ev[]
+  Presumably the intention was to rewrite the term ~c[(stp st)] when the
+  ~c[fld1] component of ~c[st] is seen to be an explicit constant.  As
+  explained elsewhere (~pl[free-variables]), we can obtain the result of
+  rewriting ~c[(fld1 st)] by binding a fresh variable to that term using
+  ~c[EQUAL], as follows.
+  ~bv[]
+    (defthm good
+      (implies (and (equal f (fld1 st))
+                    (syntaxp (quotep f)))
+               (equal (stp st)
+                      (and (true-listp st)
+                           (equal (len st) 2)
+                           (fld1p (car st))))))
+  ~ev[]
+  The event above is admitted by ACL2.  We can see it in action by disabling
+  the definition of ~c[stp] so that only the rule above, ~c[good], is available
+  for reasoning about ~c[stp].
+  ~bv[]
+    (in-theory (disable stp))
+  ~ev[]
+  Then the proof fails for the following, because the ~c[syntaxp] hypothesis of
+  the rule, ~c[good], fails: ~c[(quotep f)] evaluates to ~c[nil] when ~c[f] is
+  bound to the term ~c[(fld1 st)].
+  ~bv[]
+    (thm (stp st))
+  ~ev[]
+  However, the proof succeeds for the next form, as we explain below.
+  ~bv[]
+    (thm (stp (list 3 rest)))
+  ~ev[]
+  Consider what happens in that case when rule ~c[good] is applied to the term
+  ~c[(stp (list 3 rest))].  (~l[free-variables] for relevant background.)  The
+  first hypothesis of ~c[good] binds the variable ~c[f] to the result of
+  rewriting ~c[(fld1 st)], where ~c[st] is bound to the (internal form of) the
+  term ~c[(list 3 rest)] ~-[] and that result is clearly the term, ~c['3].
+  Then the ~c[syntaxp] hypothesis is successfully relieved, because the
+  evaluation of ~c[(quotep f)] returns ~c[t] in the environment that binds
+  ~c[f] to ~c['3]."
 
   `(synp (quote nil) (quote (syntaxp ,form)) (quote (and ,form t))))
 
